Added better support for polymorphic bindings

theories/models/utp_simple.thy
@@ -1,5 +1,7 @@
 theory utp_simple
-imports utp_base Derive
+imports 
+  utp_base 
+  Derive
 begin
 
 datatype SimpT = NtT | BlT
@@ -91,20 +93,316 @@ fun liftNBF :: "(nat \<Rightarrow> nat \<Rightarrow> bool) \<Rightarrow> SimpV \
 "liftNBF f (NtV x) (NtV y) = BlV (f x y)" |
 "liftNBF f _ _ = UdV BlT"
 
-fun sem_svar :: "svar \<Rightarrow> SimpV VAR" where
-"sem_svar (n,t) = MkPlain n (embTYPE t) False"
+fun sem_svar :: "svar \<Rightarrow> SimpV VAR" ("\<lbrakk>_\<rbrakk>\<^sub>v") where
+"\<lbrakk>(n,t)\<rbrakk>\<^sub>v = MkPlain n (embTYPE t) False"
 
-fun sem_SimpE :: "SimpE \<Rightarrow> SimpV WF_EXPRESSION" where
-"sem_SimpE (LiE v) = LitE v" |
-"sem_SimpE (PlE x y) = Op2E (liftNNF (op +)) (sem_SimpE x) (sem_SimpE y)" |
-"sem_SimpE (MlE x y) = Op2E (liftNNF (op *)) (sem_SimpE x) (sem_SimpE y)" |
-"sem_SimpE (LqE x y) = Op2E (liftNBF (op \<le>)) (sem_SimpE x) (sem_SimpE y)" |
-"sem_SimpE (VrE v) = VarE (sem_svar v)"
+fun sem_SimpE :: "SimpE \<Rightarrow> SimpV WF_EXPRESSION" ("\<lbrakk>_\<rbrakk>\<^sub>e") where
+"\<lbrakk>LiE v\<rbrakk>\<^sub>e = LitE v" |
+"\<lbrakk>PlE x y\<rbrakk>\<^sub>e = Op2E (liftNNF (op +)) \<lbrakk>x\<rbrakk>\<^sub>e \<lbrakk>y\<rbrakk>\<^sub>e" |
+"\<lbrakk>MlE x y\<rbrakk>\<^sub>e = Op2E (liftNNF (op *)) \<lbrakk>x\<rbrakk>\<^sub>e \<lbrakk>y\<rbrakk>\<^sub>e" |
+"\<lbrakk>LqE x y\<rbrakk>\<^sub>e = Op2E (liftNBF (op \<le>)) \<lbrakk>x\<rbrakk>\<^sub>e \<lbrakk>y\<rbrakk>\<^sub>e" |
+"\<lbrakk>VrE v\<rbrakk>\<^sub>e = VarE \<lbrakk>v\<rbrakk>\<^sub>v"
 
-fun sem_SimpP :: "SimpP \<Rightarrow> SimpV WF_PREDICATE" where
-"sem_SimpP SkP = II" |
-"sem_SimpP (SqP P Q) = (sem_SimpP P) ; (sem_SimpP Q)" |
-"sem_SimpP (AsP x e) = (sem_svar x) :=\<^sub>R (sem_SimpE e)" |
-"sem_SimpP (WhP e P) = IterP (ExprP (sem_SimpE e)) (sem_SimpP P)"
+fun sem_SimpP :: "SimpP \<Rightarrow> SimpV WF_PREDICATE" ("\<lbrakk>_\<rbrakk>\<^sub>p") where
+"\<lbrakk>SkP\<rbrakk>\<^sub>p = II" |
+"\<lbrakk>SqP P Q\<rbrakk>\<^sub>p = \<lbrakk>P\<rbrakk>\<^sub>p ; \<lbrakk>Q\<rbrakk>\<^sub>p" |
+"\<lbrakk>AsP x e\<rbrakk>\<^sub>p = \<lbrakk>x\<rbrakk>\<^sub>v :=\<^sub>R \<lbrakk>e\<rbrakk>\<^sub>e" |
+"\<lbrakk>WhP e P\<rbrakk>\<^sub>p = IterP (ExprP \<lbrakk>e\<rbrakk>\<^sub>e) \<lbrakk>P\<rbrakk>\<^sub>p"
+
+abbreviation "nv \<equiv> MkPlainP ''pv'' False TYPE(int) TYPE('m :: INT_SORT)"
+
+lemma "`nv := \<guillemotleft>5\<guillemotright>; nv := $nv * \<guillemotleft>5\<guillemotright>` = `nv := \<guillemotleft>25\<guillemotright>`"
+  apply (utp_rel_tac)
+  apply (auto simp add: EvalR_AssignR_typed evalp closure typing defined unrest relcomp_unfold)
+done
+
+abbreviation "nv1 \<equiv> MkPlainP ''nv1'' False TYPE(int) TYPE('m :: INT_SORT)"
+abbreviation "nv2 \<equiv> MkPlainP ''nv2'' False TYPE(int) TYPE('m :: INT_SORT)"
+
+theorem SubstP_rel_UNDASHED_ty [evalr] :
+  fixes x :: "('a :: DEFINED, 'm :: VALUE) PVAR"
+  assumes 
+    "TYPEUSOUND('a, 'm)"
+    "x \<in> PUNDASHED" 
+    "e \<rhd>\<^sub>* x" 
+    "DASHED \<sharp> e"
+  shows "\<lbrakk>p[e\<down>/\<^sub>px\<down>]\<rbrakk>R = {(b1, b2) | b1 b2. (b1(x :=\<^sub>* \<lbrakk>e\<rbrakk>\<^sub>*b1), b2) \<in> \<lbrakk>p\<rbrakk>R}"
+  apply (subst SubstP_rel_UNDASHED)
+  apply (simp_all add:evale typing closure defined assms unrest binding_upd_ty_def)
+done
+
+theorem AssignR_SemiR_ty:
+  fixes x :: "('a :: DEFINED, 'm :: VALUE) PVAR"
+  assumes 
+    "TYPEUSOUND('a, 'm)"
+    "x \<in> PUNDASHED" 
+    "e \<rhd>\<^sub>* x" 
+    "DASHED \<sharp> e"
+  shows "`(x := e) ; p` = `p[e/x]`"
+  apply (utp_rel_tac)
+  apply (simp add: EvalR_AssignR_typed evalp closure typing defined unrest relcomp_unfold assms SubstP_rel_UNDASHED_ty)
+  apply (auto simp add: binding_upd_ty_def)
+  apply (metis InjU_EvalPE_compat PVAR_VAR_PUNDASHED_UNDASHED WF_REL_BINDING_binding_upd_remove WF_REL_BINDING_member1 assms(2) assms(3))
+done
+
+lemma [simp]: "(x::int) < y \<Longrightarrow> `<x> < <y>` = true"
+  by (simp add:eval)
+
+lemma [simp]: "\<not> (x::int) < y \<Longrightarrow> `<x> < <y>` = false"
+  by (simp add:eval)
+
+lemma [simp]: "|<x :: int> + <y>| = |<x + y>|"
+  by (simp add:evalp)
+
+abbreviation 
+  "prog1 \<equiv> `while ($nv1 < \<guillemotleft>5\<guillemotright>) do 
+              (nv1 := $nv1 + \<guillemotleft>1\<guillemotright>)
+            od`"
+ 
+abbreviation "fv \<equiv> MkPlainP ''fact'' False TYPE(int) TYPE('m :: INT_SORT)"
+abbreviation "cv \<equiv> MkPlainP ''c'' False TYPE(int) TYPE('m :: INT_SORT)"
+
+type_synonym 'a WF_STATE = "('a WF_PREDICATE * 'a WF_PREDICATE)"
+
+fun StepP :: "'a WF_STATE \<Rightarrow> 'a WF_STATE \<Rightarrow> bool" (infix "~>" 50) where
+"(s,P) ~> (t,Q) \<longleftrightarrow> (s\<acute>;P) \<sqsubseteq> (t\<acute>;Q)"
+
+lemma SkipR_step:
+  "(s, II; P) ~> (s, P)"
+  by simp
+
+lemma SeqR_step:
+  "(s,P) ~> (t,P') \<Longrightarrow> (s, P;Q) ~> (t, P';Q)"
+  apply (simp)
+  apply (simp add:SemiR_assoc)
+  apply (rule refine)
+  apply (assumption)
+  apply (rule order_refl)
+done
+
+lemma ChoiceP_step1:
+  "(s, P \<sqinter> Q) ~> (s, P)"
+  apply (simp)
+  apply (metis RefineP_choice1 SemiR_mono_refine order_refl)
+done
+
+lemma ChoiceP_step2:
+  "(s, P \<sqinter> Q) ~> (s, Q)"
+  apply (simp)
+  apply (metis RefineP_choice2 SemiR_mono_refine order_refl)
+done
+
+lemma UNREST_SemiR_UNDASHED [unrest]:
+  "\<lbrakk> vs \<sharp> P; vs \<subseteq> UNDASHED; P \<in> WF_RELATION; Q \<in> WF_RELATION \<rbrakk> \<Longrightarrow> vs \<sharp> (P ; Q)"
+  apply (simp add:SemiR_algebraic_rel)
+  apply (rule unrest)
+  apply (rule unrest)
+  apply (rule unrest)
+  apply (simp)
+  apply (simp add:urename)
+  apply (rule unrest)
+  apply (simp add:WF_RELATION_def)
+  apply (auto simp add:urename)
+done
+
+lemma UNREST_SemiR_DASHED [unrest]:
+  "\<lbrakk> vs \<sharp> Q; vs \<subseteq> DASHED; P \<in> WF_RELATION; Q \<in> WF_RELATION \<rbrakk> \<Longrightarrow> vs \<sharp> (P ; Q)"
+  apply (simp add:SemiR_algebraic_rel)
+  apply (rule unrest)
+  apply (rule unrest)
+  apply (rule unrest)
+  apply (simp add:WF_RELATION_def)
+  apply (auto simp add:urename)
+  apply (rule unrest)
+  apply (simp)
+  apply (simp add:urename)
+done
+
+lemma WF_RELATION_CONDITION_true: 
+  assumes "P \<in> WF_RELATION" "(P ; true) = P"
+  shows "P \<in> WF_CONDITION"
+proof -
+  have "D\<^sub>1 \<sharp> (P ; true)"
+    by (simp add:unrest closure assms(1))
+
+  thus ?thesis
+    by (simp add:WF_CONDITION_def assms)
+qed
+
+lemma WF_RELATION_POSTCOND_true: 
+  assumes "P \<in> WF_RELATION" "(true ; P) = P"
+  shows "P \<in> WF_POSTCOND"
+proof -
+  have "D\<^sub>0 \<sharp> (true ; P)"
+    by (simp add:unrest closure assms(1))
+
+  thus ?thesis
+    by (simp add:WF_POSTCOND_def assms)
+qed
+
+lemma SemiR_first_POSTCOND [closure]:
+  "\<lbrakk> p \<in> WF_POSTCOND; Q \<in> WF_RELATION \<rbrakk> \<Longrightarrow> p ; Q \<in> WF_POSTCOND"
+  by (metis (full_types) SemiR_TrueP_postcond SemiR_assoc SemiR_closure WF_POSTCOND_WF_RELATION WF_RELATION_POSTCOND_true)
+
+lemma SemiR_second_CONDITION [closure]:
+  "\<lbrakk> P \<in> WF_RELATION; q \<in> WF_CONDITION \<rbrakk> \<Longrightarrow> P ; q \<in> WF_CONDITION"
+  by (metis SemiR_TrueP_precond SemiR_assoc SemiR_closure WF_CONDITION_WF_RELATION WF_RELATION_CONDITION_true)
+
+definition uv :: 
+  "'a WF_PREDICATE \<Rightarrow> ('a VAR) set" where
+"uv p = \<Union> {vs. UNREST vs p}"
+
+lemma UNREST_uv_upper: 
+  "xs \<sharp> P \<Longrightarrow> xs \<subseteq> uv P"
+  by (auto simp add:uv_def)
+
+lemma UNREST_uv_least:
+  "(\<And>xs. xs \<sharp> P \<Longrightarrow> xs \<subseteq> zs) \<Longrightarrow> uv P \<subseteq> zs"
+  by (auto simp add:uv_def)
+
+lemma "\<lbrakk> \<forall> x \<in> xs. {x} \<sharp> P \<rbrakk> \<Longrightarrow> xs \<sharp> (P :: 'a WF_PREDICATE)"
+  apply (subgoal_tac "(\<forall>x\<in>xs. \<forall>b1\<in>destPRED P. \<forall>b2. b1(x :=\<^sub>b \<langle>b2\<rangle>\<^sub>b x) \<in> destPRED P) 
+       \<longleftrightarrow> (\<forall>b1\<in>destPRED P. \<forall>b2. \<forall>x\<in>xs. b1(x :=\<^sub>b \<langle>b2\<rangle>\<^sub>b x) \<in> destPRED P)")
+  apply (auto simp add:UNREST_def)
+  apply (drule_tac x="b1" in bspec, simp)
+  apply (drule_tac x="b2" in spec)
+
+proof -
+  have 
+    by (auto)
+  apply (simp add:binding_override_on_def)
+
+lemma UNREST_uv_upper: 
+  "xs \<sharp> P \<longleftrightarrow> xs \<subseteq> uv P"
+  apply (auto simp add:uv_def)
+  apply (auto simp add:subset_eq)
+  apply (auto simp add:UNREST_def)
+  apply (auto simp add:binding_override_on_def override_on_def)
+
+
+done
+
+(*
+lemma 
+  fixes P :: "'a WF_PREDICATE"
+  assumes "\<forall>vs\<in>vss. vs \<sharp> P"
+  shows "(\<Union> vss) \<sharp> P"
+  using assms
+  apply (auto simp add:UNREST_def binding_override_on_def override_on_def)
+  apply (auto simp add:)
+  apply (rule) back back back
+  apply (drule bspec)
+  defer
+*)
+
+lemma "uv P \<sharp> P"
+  apply (simp add:uv_def)
+
+
+
+
+lemma 
+  assumes 
+    "s \<in> WF_POSTCOND"
+    "P \<in> WF_RELATION"
+    "Q \<in> WF_RELATION"
+  shows "`s ; (P \<and> Q)` = `(s ; P) \<and> (s ; Q)`"
+  apply (simp add:closure SemiR_algebraic_rel assms urename)
+proof -
+  have "`s ; (P \<and> Q)` = `true ; (s\<acute> \<and> P \<and> Q)`"
+    by (metis AndP_rel_closure SemiR_AndP_left_postcond TrueP_rel_closure assms(1) assms(2) assms(3) utp_pred_simps(6))
+
+  have "... = `true ; ((s\<acute> \<and> P) \<and> (s\<acute> \<and> Q))`"
+    by (smt AndP_comm AndP_idem AndP_assoc)
+
+  using assms
+  
+
+  apply (frule_tac SemiR_TrueP_postcond)
+  apply (utp_xrel_auto_tac)
+  apply (utp_rel_auto_tac)
+
+lemma CondR_true_step:
+  "[s\<acute>;b] \<Longrightarrow> (s, P \<lhd> b \<rhd> Q) ~> (s, P)"
+  apply (simp add:CondR_def SemiR_OrP_distl)
+  apply (utp_rel_auto_tac)
+  apply (rule refine)
+
+  by (simp)
+
+lemma CondR_false_step:
+  "[\<not>(s\<acute>;b)] \<Longrightarrow> (s, P \<lhd> b \<rhd> Q) ~> (s, Q)"
+  by (simp)
+
+
+abbreviation 
+  "fact_prog \<equiv> 
+     `cv := \<guillemotleft>0\<guillemotright>; fv := \<guillemotleft>0\<guillemotright>; while ($cv \<le> $nv) do ((fv := $fv * $cv); (cv := $cv + \<guillemotleft>1\<guillemotright>)) od`"
+
+lemma "`nv1 := \<guillemotleft>0\<guillemotright> ; prog1` = `nv1 := \<guillemotleft>5\<guillemotright>`"
+  apply (subst AssignR_SemiR_ty)
+  apply (simp_all add:typing defined closure unrest)
+  apply (subst IterP_unfold)
+  apply (simp_all add:typing defined closure unrest usubst CondR_true AssignR_SemiR_ty)
+  apply (subst IterP_unfold)
+  apply (simp_all add:typing defined closure unrest usubst CondR_true AssignR_SemiR_ty)
+  apply (subst IterP_unfold)
+  apply (simp_all add:typing defined closure unrest usubst CondR_true AssignR_SemiR_ty)
+  apply (subst IterP_unfold)
+  apply (simp_all add:typing defined closure unrest usubst CondR_true AssignR_SemiR_ty)
+  apply (subst IterP_unfold)
+  apply (simp_all add:typing defined closure unrest usubst CondR_true AssignR_SemiR_ty)
+  apply (subst IterP_unfold)
+  apply (simp_all add:typing defined closure unrest usubst CondR_false AssignR_SemiR_ty)
+done
+
+
+lemma "`nv := \<guillemotleft>1\<guillemotright>; fact_prog` = undefined"
+  apply (simp add:AssignR_SemiR_ty typing defined closure unrest)
+  apply (subst IterP_unfold)
+  apply (simp add:typing defined closure unrest usubst CondR_true AssignR_SemiR_ty)
+  apply (simp add:typing defined closure unrest usubst CondR_true AssignR_SemiR_ty)
+  apply (simp add:typing defined closure unrest usubst)
+
+
+lemma "`nv1 := \<guillemotleft>0\<guillemotright> ; prog1` = `nv1 := \<guillemotleft>5\<guillemotright>`"
+  apply (subst AssignR_SemiR_ty)
+  apply (simp_all add:typing defined closure unrest)
+  apply (subst IterP_unfold)
+  apply (simp_all add:typing defined closure unrest usubst CondR_true AssignR_SemiR_ty)
+  apply (subst IterP_unfold)
+  apply (simp_all add:typing defined closure unrest usubst CondR_true AssignR_SemiR_ty)
+  apply (subst IterP_unfold)
+  apply (simp_all add:typing defined closure unrest usubst CondR_true AssignR_SemiR_ty)
+  apply (subst IterP_unfold)
+  apply (simp_all add:typing defined closure unrest usubst CondR_true AssignR_SemiR_ty)
+  apply (subst IterP_unfold)
+  apply (simp_all add:typing defined closure unrest usubst CondR_true AssignR_SemiR_ty)
+  apply (subst IterP_unfold)
+  apply (simp_all add:typing defined closure unrest usubst CondR_false AssignR_SemiR_ty)
+done
+
+
+
+
+  apply (subst SubstP_AssignR_simple)
+  apply (simp_all add
+  apply (subst usubst) back back back
+  apply (subgoal_tac "|<0 :: int> < <5>| = (|true| :: (bool, 'a) WF_PEXPRESSION)")
+  apply (simp)
+
+  thm AssignR_one_point
+
+
+  apply (utp_rel_tac)
+  apply (simp add: EvalR_AssignR_typed evalp closure typing defined unrest relcomp_unfold)
+  apply (simp add: evalr closure typing defined)
+
+
+lemma "\<lbrakk>SqP (AsP (''x'', NtT) (LiE (NtV 5))) (AsP (''x'', NtT) (LiE (NtV 6)))\<rbrakk>\<^sub>p =
+       \<lbrakk>AsP (''x'', NtT) (LiE (NtV 6))\<rbrakk>\<^sub>p"
+  apply (auto simp add:evale evalr typing defined unrest relcomp_unfold)
+  apply (subst EvalR_AssignR)
+  apply (simp_all add:typing defined closure unrest)
 
 end
