theories/poly/utp_poly_binding.thy
@@ -1,0 +1,76 @@
+(******************************************************************************)
+(* Project: Unifying Theories of Programming in HOL                           *)
+(* File: utp_poly_binding.thy                                                 *)
+(* Author: Simon Foster and Frank Zeyda, University of York (UK)              *)
+(******************************************************************************)
+
+header {* Typed Bindings *}
+
+theory utp_poly_binding
+imports 
+  "../core/utp_binding"
+  "../tactics/utp_rel_tac"
+  utp_poly_var
+begin
+
+definition Rep_binding_ty :: 
+  "'m WF_BINDING \<Rightarrow> ('a :: DEFINED, 'm :: VALUE) PVAR \<Rightarrow> 'a" ("\<langle>_\<rangle>\<^sub>*") where
+"Rep_binding_ty b x = ProjU (\<langle>b\<rangle>\<^sub>b x\<down>)"
+
+definition binding_upd_ty :: 
+  "'m WF_BINDING \<Rightarrow>
+   ('a :: DEFINED, 'm :: VALUE) PVAR \<Rightarrow>
+   'a \<Rightarrow>
+   'm WF_BINDING" where
+"binding_upd_ty b x v = binding_upd b (x\<down>) (InjU v)"
+
+nonterminal tbupdbinds and tbupdbind
+
+syntax
+  "_tbupdbind" :: "['a, 'a] => tbupdbind"               ("(2_ :=\<^sub>*/ _)")
+  ""         :: "tbupdbind => tbupdbinds"               ("_")
+  "_tbupdbinds":: "[tbupdbind, tbupdbinds] => tbupdbinds" ("_,/ _")
+  "_TBUpdate"  :: "['a, tbupdbinds] => 'a"              ("_/'((_)')" [1000, 0] 900)
+
+translations
+  "_TBUpdate f (_tbupdbinds b bs)" == "_TBUpdate (_TBUpdate f b) bs"
+  "f(x:=\<^sub>*y)" == "CONST binding_upd_ty f x y"
+
+(* Note: ProjU (InjU v) effectively performs a cast and will yield v when applied
+   to identical sound types. *)
+
+lemma binding_upd_apply_ty [simp]: 
+  fixes x :: "('a :: DEFINED , 'm :: VALUE) PVAR"
+  and   y :: "('b :: DEFINED, 'm) PVAR"
+  assumes "v \<rhd>\<^sub>p x"
+  shows "\<langle>f(x:=\<^sub>*v)\<rangle>\<^sub>* y = (if (x\<down>)=(y\<down>) then ProjU (InjU v :: 'm) else \<langle>f\<rangle>\<^sub>* y)"
+  by (auto simp add:Rep_binding_ty_def binding_upd_ty_def typing assms)
+
+lemma binding_upd_upd_ty [simp]: 
+  fixes x :: "('a :: DEFINED , 'm :: VALUE) PVAR"
+  assumes "TYPEUSOUND('a, 'm)" "y \<rhd>\<^sub>p x" "z \<rhd>\<^sub>p x"
+  shows "f(x:=\<^sub>*y,x:=\<^sub>*z) = f(x:=\<^sub>*z)"
+  apply (simp add:binding_upd_ty_def)
+  apply (subst binding_upd_upd)
+  apply (simp_all add:typing defined assms)
+done
+
+lemma WF_REL_BINDING_binding_upd_ty [closure]: 
+  fixes x :: "('a :: DEFINED, 'm :: VALUE) PVAR"
+  assumes "TYPEUSOUND('a, 'm)" "x \<in> PUNDASHED" "v \<rhd>\<^sub>p x" "b \<in> WF_REL_BINDING"
+  shows "b(x :=\<^sub>* v) \<in> WF_REL_BINDING"
+  apply (simp add:binding_upd_ty_def closure assms)
+  apply (rule closure)
+  apply (metis PVAR_VAR_PUNDASHED_UNDASHED assms)
+  apply (simp_all add:assms)
+  apply (rule typing)
+  apply (simp_all add:assms)
+done
+
+lemma Rep_WF_BINDING_ty_pvaux_defined [defined]:
+  fixes x :: "('a :: DEFINED, 'm :: VALUE) PVAR"
+  assumes "TYPEUSOUND('a, 'm)" "pvaux x"
+  shows "\<D> (\<langle>b\<rangle>\<^sub>* x)"
+  by (auto intro:defined typing assms simp add:Rep_binding_ty_def)
+
+end
